## 156. Binary Tree Upside Down

Given a binary tree where all the right nodes are either leaf nodes with a sibling (a left node that shares the same parent node) or empty, flip it upside down and turn it into a tree where the original right nodes turned into left leaf nodes. Return the new root.


### Example
```
Input: [1,2,3,4,5]

    1
   / \
  2   3
 / \
4   5

Output: return the root of the binary tree [4,5,2,#,#,3,1]

   4
  / \
 5   2
    / \
   3   1  

```

### My Code
```c++
/**
 * Definition for a binary tree node.
 * struct TreeNode {
 *     int val;
 *     TreeNode *left;
 *     TreeNode *right;
 *     TreeNode(int x) : val(x), left(NULL), right(NULL) {}
 * };
 */
class Solution {
public:
    TreeNode* upsideDownBinaryTree(TreeNode* root) {
        if(!root || !root->left)
            return root;
        TreeNode* cur_left = root->left;
        TreeNode* cur_right = root->right;
        
        TreeNode* new_root = upsideDownBinaryTree(root->left);

        cur_left->right = root;
        cur_left->left = cur_right;
        root->left = nullptr;
        root->right = nullptr;
        
        return new_root;
    }
};
```
相當於把樹的節點順時針繞一遍，
當前的樹的最左子樹點會變成新的root
recursive回傳新的new root 再依序把當前的root變成右子樹，當前的右子樹變左子樹

### Others Solution
```c++
// Recursion
class Solution {
public:
    TreeNode *upsideDownBinaryTree(TreeNode *root) {
        if (!root || !root->left) return root;
        TreeNode *l = root->left, *r = root->right;
        TreeNode *res = upsideDownBinaryTree(l);
        l->left = r;
        l->right = root;
        root->left = NULL;
        root->right = NULL;
        return res;
    }
};


// Iterative
class Solution {
public:
    TreeNode *upsideDownBinaryTree(TreeNode *root) {
        TreeNode *cur = root, *pre = NULL, *next = NULL, *tmp = NULL;
        while (cur) {
            next = cur->left;
            cur->left = tmp;
            tmp = cur->right;
            cur->right = pre;
            pre = cur;
            cur = next;
        }
        return pre;
    }
};
```

