## 779. K-th Symbol in Grammar

On the first row, we write a 0. Now in every subsequent row, we look at the previous row and replace each occurrence of 0 with 01, and each occurrence of 1 with 10.

Given row N and index K, return the K-th indexed symbol in row N. (The values of K are 1-indexed.) (1 indexed).


### Example
```
Examples:
Input: N = 1, K = 1
Output: 0

Input: N = 2, K = 1
Output: 0

Input: N = 2, K = 2
Output: 1

Input: N = 4, K = 5
Output: 1

Explanation:
row 1: 0
row 2: 01
row 3: 0110
row 4: 01101001
```

### My Code
```c++
class Solution {
public:
    int kthGrammar(int N, int K) {
        if(N == 1)
            return 0;
        
        if(K % 2 == 0)
            return (kthGrammar(N-1, K/2) == 0 ? 1 : 0);
        else
            return (kthGrammar(N-1, (K+1)/2) == 0 ? 0 : 1);
    }
};
```
time complexity : O(N)

### Others Solution
```c++
int kthGrammar(int N, int K) {
    int n;
    for (n = 0, K -= 1; K ; K &= (K - 1)) n++;
    return n & 1;
}
```
First, you can easily find that prefix of every row is exactly the same.
It not difficult to understand.
Beacause every 2 * L fisrt letters are generated by the same L fist letters.

Then, we know that every row is the start part of the same long sequence.
Moreover K is guaranteed to be an integer in the range[1, 2 ^ (N - 1)].
So result depends only on value K

Suppose 2 ^ L < K <= 2 ^ (L + 1).
2 ^ (L - 1) is the biggest 2's power smaller than K.
Kth number is generated from K - 2 ^ (L - 1)
Kth number is also different from K - 2 ^ (L - 1)
So we toggle K to K - 2 ^ L by subtracting 2 ^ L

We repeat the process until we toggle K to 1, which mean we need to substract K - 1 in total.
What we should do is transfer K - 1 in binary so that we can easily find how many times we need to toggle.

